<?xml version="1.0" encoding="UTF-8"?>
<rdf:RDF
	xmlns="http://www.w3.org/ns/lemon/termlex#"
	xmlns:grddl="http://www.w3.org/2003/g/data-view#"
	xmlns:rdf="http://www.w3.org/1999/02/22-rdf-syntax-ns#"
	xmlns:owl="http://www.w3.org/2002/07/owl#"
	xmlns:xsd="http://www.w3.org/2001/XMLSchema#"
	xmlns:rdfs="http://www.w3.org/2000/01/rdf-schema#"
	xmlns:cc="http://creativecommons.org/ns#"
	xmlns:dc="http://purl.org/dc/elements/1.1/"
	xmlns:dcterms="http://purl.org/dc/terms/">

<rdf:Description rdf:about="http://www.w3.org/ns/lemon/termlex">
	<rdf:type rdf:resource="http://www.w3.org/2002/07/owl#Ontology"/>
	<owl:imports rdf:resource="http://www.w3.org/ns/lemon/ontolex"/>
	<owl:imports rdf:resource="http://www.w3.org/2004/02/skos/core"/>
	<dc:title xml:lang="en">Termlex Extension for Terminologies</dc:title>
	<dc:contributor xml:lang="en">Patricia Martín-Chozas</dc:contributor>
	<dc:contributor xml:lang="en">Thierry Declerck</dc:contributor>
	<dc:contributor xml:lang="en">Elena Montiel-Ponsoda</dc:contributor>
	<dc:contributor xml:lang="en">Víctor Rodríguez-Doncel</dc:contributor>
	<cc:licence rdf:resource="https://creativecommons.org/publicdomain/zero/1.0/"/>
	<dcterms:license rdf:resource="https://creativecommons.org/publicdomain/zero/1.0/"/>
</rdf:Description>

<rdf:Description rdf:about="http://www.w3.org/ns/lemon/termlex#Definition">
	<rdf:type rdf:resource="http://www.w3.org/2002/07/owl#Class"/>
	<rdfs:subClassOf rdf:resource="http://www.w3.org/2002/07/owl#Thing"/>
	<rdfs:label xml:lang="en">Definition</rdfs:label>
	<rdfs:comment xml:lang="en">The Definition class represents the description of a resource, may it be a concept, a term or any other entity. Additional information can be attached to it, such as the source and authorship of the definition.</rdfs:comment>
</rdf:Description>

<rdf:Description rdf:about="http://www.w3.org/ns/lemon/termlex#Note">
	<rdf:type rdf:resource="http://www.w3.org/2002/07/owl#Class"/>
	<rdfs:subClassOf rdf:resource="http://www.w3.org/2002/07/owl#Thing"/>
	<rdfs:label xml:lang="en">Note</rdfs:label>
	<rdfs:comment xml:lang="en">The Note class represents additional information given about a resource, may it be a concept, a term or any other entity. Oher data can be attached to it, such as the source and authorship of the note.</rdfs:comment>
</rdf:Description>

<rdf:Description rdf:about="http://www.w3.org/ns/lemon/termlex#Source">
	<rdf:type rdf:resource="http://www.w3.org/2002/07/owl#Class"/>
	<rdfs:subClassOf rdf:resource="http://www.w3.org/2002/07/owl#Thing"/>
	<rdfs:label xml:lang="en">Source</rdfs:label>
	<rdfs:comment xml:lang="en">The Source class represents the provenance information of an element, may it be the authorship, notes or other sources.</rdfs:comment>
</rdf:Description>

<rdf:Description rdf:about="http://www.w3.org/ns/lemon/termlex#ReliabilityCode">
	<rdf:type rdf:resource="http://www.w3.org/2002/07/owl#Class"/>
	<rdfs:subClassOf rdf:resource="http://www.w3.org/2002/07/owl#Thing"/>
	<rdfs:label xml:lang="en">Reliability Code</rdfs:label>
	<rdfs:comment xml:lang="en">The ReliabilityCode class represents the trustworthiness degree of a determined resource, may it be a concept, a term or any other entity. This class points at a fixed set of values, from 1 to 5, for standardisation purposes.
</rdfs:comment>
	<rdf:value rdf:resource="http://www.w3.org/ns/lemon/termlex#1"/>
	<rdf:value rdf:resource="http://www.w3.org/ns/lemon/termlex#2"/>
	<rdf:value rdf:resource="http://www.w3.org/ns/lemon/termlex#3"/>
	<rdf:value rdf:resource="http://www.w3.org/ns/lemon/termlex#4"/>
	<rdf:value rdf:resource="http://www.w3.org/ns/lemon/termlex#5"/>
</rdf:Description>

<rdf:Description rdf:about="http://www.w3.org/ns/lemon/termlex#1">
	<rdf:type rdf:resource="http://www.w3.org/ns/lemon/termlex#ReliabilityCode"/>
</rdf:Description>

<rdf:Description rdf:about="http://www.w3.org/ns/lemon/termlex#2">
	<rdf:type rdf:resource="http://www.w3.org/ns/lemon/termlex#ReliabilityCode"/>
</rdf:Description>

<rdf:Description rdf:about="http://www.w3.org/ns/lemon/termlex#3">
	<rdf:type rdf:resource="http://www.w3.org/ns/lemon/termlex#ReliabilityCode"/>
</rdf:Description>

<rdf:Description rdf:about="http://www.w3.org/ns/lemon/termlex#4">
	<rdf:type rdf:resource="http://www.w3.org/ns/lemon/termlex#ReliabilityCode"/>
</rdf:Description>

<rdf:Description rdf:about="http://www.w3.org/ns/lemon/termlex#5">
	<rdf:type rdf:resource="http://www.w3.org/ns/lemon/termlex#ReliabilityCode"/>
</rdf:Description>

<rdf:Description rdf:about="http://www.w3.org/ns/lemon/termlex#Usage">
	<rdf:type rdf:resource="http://www.w3.org/2002/07/owl#Class"/>
	<rdfs:subClassOf rdf:resource="http://www.w3.org/2002/07/owl#Thing"/>
	<rdfs:label xml:lang="en">Usage</rdfs:label>
	<rdfs:comment xml:lang="en">The Usage class represents usage notes, advices or indications regarding the lexical sense of a given terminological concept. </rdfs:comment>
</rdf:Description>

<rdf:Description rdf:about="http://www.w3.org/ns/lemon/termlex#TerminologicalConcept">
	<rdf:type rdf:resource="http://www.w3.org/2002/07/owl#Class"/>
	<rdfs:subClassOf rdf:resource="http://www.w3.org/2002/07/owl#Thing"/>
	<rdfs:subClassOf rdf:resource="http://www.w3.org/2004/02/skos/core#Concept"/>
	<rdfs:label xml:lang="en">Terminological Concept</rdfs:label>
	<rdfs:comment xml:lang="en">The TerminologicalConcept class represents a mental abstraction, concept or unit of thought that embodies the meaning of one or more lexical entries, that refer to the same lexical sense, thus, belong to the same area of epertise.</rdfs:comment>
</rdf:Description>

<rdf:Description rdf:about="http://www.w3.org/ns/lemon/termlex#isEvokedBy">
	<rdf:type rdf:resource="http://www.w3.org/2002/07/owl#ObjectProperty"/>
	<rdfs:label xml:lang="en">is evoked by</rdfs:label>
	<rdfs:comment xml:lang="en">The isEvokedBy property relates a terminological concept to one of the lexical entries that evoke it.</rdfs:comment>
	<rdfs:range rdf:resource="http://www.w3.org/ns/lemon/ontolex#LexicalEntry"/>
	<rdfs:domain rdf:resource="http://www.w3.org/ns/lemon/termlex#TerminologicalConcept"/>
</rdf:Description>

<rdf:Description rdf:about="http://www.w3.org/ns/lemon/termlex#lexicalizedSense">
	<rdf:type rdf:resource="http://www.w3.org/2002/07/owl#ObjectProperty"/>
	<rdf:type rdf:resource="http://www.w3.org/2002/07/owl#FunctionalProperty"/>
	<rdfs:label xml:lang="en">lexicalized sense</rdfs:label>
	<rdfs:comment xml:lang="en">The lexicalizedSense property relates a terminological concept to a unique corresponding lexical sense.</rdfs:comment>
	<rdfs:range rdf:resource="http://www.w3.org/ns/lemon/ontolex#LexicalSense"/>
	<rdfs:domain rdf:resource="http://www.w3.org/ns/lemon/termlex#TerminologicalConcept"/>
	<owl:inverseOf rdf:resource="http://www.w3.org/ns/lemon/termlex#isLexicalizedSenseOf"/>
</rdf:Description>

<rdf:Description rdf:about="http://www.w3.org/ns/lemon/termlex#isLexicalizedSenseOf">
	<rdf:type rdf:resource="http://www.w3.org/2002/07/owl#ObjectProperty"/>
	<rdf:type rdf:resource="http://www.w3.org/2002/07/owl#FunctionalProperty"/>
	<rdfs:label xml:lang="en">is lexicalized sense of</rdfs:label>
	<rdfs:comment xml:lang="en">The isLexicalizedSense property relates a lexical sense to a unique corresponding terminological concept.</rdfs:comment>
	<rdfs:range rdf:resource="http://www.w3.org/ns/lemon/termlex#TerminologicalConcept"/>
	<rdfs:domain rdf:resource="http://www.w3.org/ns/lemon/ontolex#LexicalSense"/>
	<owl:inverseOf rdf:resource="http://www.w3.org/ns/lemon/termlex#lexicalizedSense"/>
</rdf:Description>

<rdf:Description rdf:about="http://www.w3.org/ns/lemon/termlex#evokes">
	<rdf:type rdf:resource="http://www.w3.org/1999/02/22-rdf-syntax-ns#Property"/>
	<rdfs:label xml:lang="en">evokes</rdfs:label>
	<rdfs:comment xml:lang="en">The evokes property relates a lexical entry to the terminological concepts it evokes.</rdfs:comment>
	<rdfs:range rdf:resource="http://www.w3.org/ns/lemon/termlex#TerminologicalConcept"/>
	<rdfs:domain rdf:resource="http://www.w3.org/ns/lemon/ontolex#LexicalEntry"/>
	<owl:inverseOf rdf:resource="http://www.w3.org/ns/lemon/termlex#isEvokedBy"/>
</rdf:Description>

<rdf:Description rdf:about="http://www.w3.org/ns/lemon/termlex#reliabilityCode">
	<rdf:type rdf:resource="http://www.w3.org/2002/07/owl#ObjectProperty"/>
	<rdfs:label xml:lang="en">Reliability Code</rdfs:label>
	<rdfs:comment xml:lang="en">The reliabilityCode property relates a lexical sense to the the reliability code class.</rdfs:comment>
	<rdfs:range rdf:resource="http://www.w3.org/ns/lemon/termlex#ReliabilityCode"/>
</rdf:Description>

<rdf:Description rdf:about="http://www.w3.org/ns/lemon/termlex#isConceptOf">
	<rdf:type rdf:resource="http://www.w3.org/2002/07/owl#ObjectProperty"/>
	<rdfs:label xml:lang="en">is concept of</rdfs:label>
	<rdfs:comment xml:lang="en">The isConceptOf property relates the meaning of a Terminological Concept by linking it to a particular ontological meaning.</rdfs:comment>
	<rdfs:domain rdf:resource="http://www.w3.org/ns/lemon/termlex#TerminologicalConcept"/>
	<owl:inverseOf rdf:resource="http://www.w3.org/ns/lemon/termlex#concept"/>
</rdf:Description>

<rdf:Description rdf:about="http://www.w3.org/ns/lemon/termlex#concept">
	<rdf:type rdf:resource="http://www.w3.org/2002/07/owl#ObjectProperty"/>
	<rdfs:label xml:lang="en">concept</rdfs:label>
	<rdfs:comment xml:lang="en">The concept property relates an ontological entity to a terminological concept that represents the corresponding meaning.</rdfs:comment>
	<rdfs:range rdf:resource="http://www.w3.org/ns/lemon/termlex#TerminologicalConcept"/>
	<owl:inverseOf rdf:resource="http://www.w3.org/ns/lemon/termlex#isConceptOf"/>
</rdf:Description>

</rdf:RDF>